\documentclass[journal,12pt,twocolumn]{IEEEtran}

\usepackage{setspace}
\usepackage{gensymb}


\singlespacing

\usepackage[cmex10]{amsmath}
%\usepackage{amsthm}
%\interdisplaylinepenalty=2500
%\savesymbol{iint}
%\usepackage{txfonts}
%\restoresymbol{TXF}{iint}
%\usepackage{wasysym}
\usepackage{amsthm}

\usepackage{mathrsfs}
\usepackage{txfonts}
\usepackage{stfloats}
\usepackage{bm}
\usepackage{cite}
\usepackage{cases}
\usepackage{subfig}

\usepackage{longtable}
\usepackage{multirow}

\usepackage{enumitem}
\usepackage{mathtools}
\usepackage{steinmetz}
\usepackage{tikz}
\usepackage{circuitikz}
\usepackage{verbatim}
\usepackage{tfrupee}
\usepackage[breaklinks=true]{hyperref}

\usepackage{tkz-euclide} %loads TikZ and tkz-base

\usetikzlibrary{calc,math}
\usepackage{listings}
    \usepackage{color}                                          
    \usepackage{array}                                          
    \usepackage{longtable}                                      
    \usepackage{calc}                                          
    \usepackage{multirow}                                      
    \usepackage{hhline}                                        
    \usepackage{ifthen}
    \usepackage{lscape}    
\usepackage{multicol}
\usepackage{chngcntr}

\DeclareMathOperator*{\Res}{Res}

\renewcommand\thesection{\arabic{section}}
\renewcommand\thesubsection{\thesection.\arabic{subsection}}
\renewcommand\thesubsubsection{\thesubsection.\arabic{subsubsection}}

\renewcommand\thesectiondis{\arabic{section}}
\renewcommand\thesubsectiondis{\thesectiondis.\arabic{subsection}}
\renewcommand\thesubsubsectiondis{\thesubsectiondis.\arabic{subsubsection}}

\hyphenation{op-tical net-works semi-conduc-tor}
\def\inputGnumericTable{}                                 %%

\lstset{
%language=C,
frame=single,
breaklines=true,
columns=fullflexible
}

\begin{document}

\newtheorem{theorem}{Theorem}[section]
\newtheorem{problem}{Problem}
\newtheorem{proposition}{Proposition}[section]
\newtheorem{lemma}{Lemma}[section]
\newtheorem{corollary}[theorem]{Corollary}
\newtheorem{example}{Example}[section]
\newtheorem{definition}[problem]{Definition}

\newcommand{\BEQA}{\begin{eqnarray}}
\newcommand{\EEQA}{\end{eqnarray}}
\newcommand{\define}{\stackrel{\triangle}{=}}
\bibliographystyle{IEEEtran}
\providecommand{\mbf}{\mathbf}
\providecommand{\pr}[1]{\ensuremath{\Pr\left(#1\right)}}
\providecommand{\qfunc}[1]{\ensuremath{Q\left(#1\right)}}
\providecommand{\sbrak}[1]{\ensuremath{{}\left[#1\right]}}
\providecommand{\lsbrak}[1]{\ensuremath{{}\left[#1\right.}}
\providecommand{\rsbrak}[1]{\ensuremath{{}\left.#1\right]}}
\providecommand{\brak}[1]{\ensuremath{\left(#1\right)}}
\providecommand{\lbrak}[1]{\ensuremath{\left(#1\right.}}
\providecommand{\rbrak}[1]{\ensuremath{\left.#1\right)}}
\providecommand{\cbrak}[1]{\ensuremath{\left\{#1\right\}}}
\providecommand{\lcbrak}[1]{\ensuremath{\left\{#1\right.}}
\providecommand{\rcbrak}[1]{\ensuremath{\left.#1\right\}}}
\theoremstyle{remark}
\newtheorem{rem}{Remark}
\newcommand{\sgn}{\mathop{\mathrm{sgn}}}
\providecommand{\abs}[1]{\left\vert#1\right\vert}
\providecommand{\res}[1]{\Res\displaylimits_{#1}}
\providecommand{\norm}[1]{\left\lVert#1\right\rVert}
%\providecommand{\norm}[1]{\lVert#1\rVert}
\providecommand{\mtx}[1]{\mathbf{#1}}
\providecommand{\mean}[1]{E\left[ #1 \right]}
\providecommand{\fourier}{\overset{\mathcal{F}}{ \rightleftharpoons}}
%\providecommand{\hilbert}{\overset{\mathcal{H}}{ \rightleftharpoons}}
\providecommand{\system}{\overset{\mathcal{H}}{ \longleftrightarrow}}
%\newcommand{\solution}[2]{\textbf{Solution:}{#1}}
\newcommand{\solution}{\noindent \textbf{Solution: }}
\newcommand{\cosec}{\,\text{cosec}\,}
\providecommand{\dec}[2]{\ensuremath{\overset{#1}{\underset{#2}{\gtrless}}}}
\newcommand{\myvec}[1]{\ensuremath{\begin{pmatrix}#1\end{pmatrix}}}
\newcommand{\mydet}[1]{\ensuremath{\begin{vmatrix}#1\end{vmatrix}}}
\numberwithin{equation}{subsection}
\makeatletter
\@addtoreset{figure}{problem}
\makeatother
\let\StandardTheFigure\thefigure
\let\vec\mathbf
\renewcommand{\thefigure}{\theproblem}
\def\putbox#1#2#3{\makebox[0in][l]{\makebox[#1][l]{}\raisebox{\baselineskip}[0in][0in]{\raisebox{#2}[0in][0in]{#3}}}}
     \def\rightbox#1{\makebox[0in][r]{#1}}
     \def\centbox#1{\makebox[0in]{#1}}
     \def\topbox#1{\raisebox{-\baselineskip}[0in][0in]{#1}}
     \def\midbox#1{\raisebox{-0.5\baselineskip}[0in][0in]{#1}}
\vspace{3cm}
\title{Assignment 4}
\author{Priya Bhatia}
\maketitle
\newpage
%\tableofcontents
\bigskip
\renewcommand{\thefigure}{\theenumi}
\renewcommand{\thetable}{\theenumi}
\begin{abstract}
This document finds the area bounded by curves
\end{abstract}
%
Download python codes from 
%
\begin{lstlisting}
https://github.com/priya6971/matrix_theory_EE5609/tree/master/Assignment4/codes
\end{lstlisting}
%
%
Download latex-tikz codes from 
%
\begin{lstlisting}
https://github.com/priya6971/matrix_theory_EE5609/tree/master/Assignment4
\end{lstlisting}
%
\section{\textbf{Problem}}
Find the area bounded by curves $\norm{\vec{x}-\myvec{1\\0}}$=1 and $\norm{\vec{x}}$=1.
\section{\textbf{Solution}}
General equation of circle is ${\vec{x}^T\vec{x}} + 2\vec{u}^T\vec{x} $+ f = 0\\
Taking equation of the first curve to be,
\begin{align}
\norm{\vec{x}-\myvec{1\\0}}^2&=1^2\\
{\vec{x}^{T}\vec{x}+2\vec{u_1}^T\vec{x}}&=0 \label{2.2.2}\\
\vec{u_1}&=\myvec{-1\\0}\\
f_1&=0\\
\vec{O_1}&=\myvec{1\\0}
\end{align}
Taking equation of the second curve to be,
\begin{align}
\norm{\vec{x}}^2 + 2\vec{u}_2^T\vec{x} + f_2&= 0\label{2.1.1}\\
{\vec{x}^{T}\vec{x}}-1&=0 \label{2.1.2}\\
\vec{u_2}&=\myvec{0\\0}\\
f_2&=-1\\
\vec{O_2}&=\myvec{0\\0}
\end{align}
Now, subtracting equation \eqref{2.2.2} from \eqref{2.1.2} We get,
\begin{align}
\vec{x}^T\vec{x}+2\vec{u_1}^T\vec{x}-\vec{x}^{T}\vec{x}-f_2&=0\\
2\vec{u}^{T}\vec{x}&=-1\\
\myvec{-2&0}\vec{x}&=-1
\end{align}
which can be written as:-
\begin{align}
\myvec{1&0}\vec{x}&=1/2 \\
\vec{x}&=\myvec{1/2 \\ 0} + \lambda \myvec{0\\1} \\
\vec{x}&=\vec{q}+\lambda\vec{m}\label{2.2.10} \\
\vec{q}&=\myvec{1/2 \\ 0} \\
\vec{m}&=\myvec{0\\1}
\end{align}
Substituting \eqref{2.2.10} in \eqref{2.1.1}
\begin{align}
\norm{\vec{x}}^2 + 2\vec{u}_2^T\vec{x} + f_2&= 0 \\
\norm{\vec{q}+\lambda\vec{m}}^2 + f_2&= 0 \\
(\vec{q}+\lambda \vec{m})^T(\vec{q}+\lambda \vec{m})+f_2&= 0 \\
\vec{q}^T(\vec{q}+\lambda \vec{m})+\lambda  \vec{m}^T(\vec{q}+\lambda \vec{m})+f_2&= 0 \\ \norm{\vec{q}}^2+\lambda\vec{q}^T\vec{m}+\lambda\vec{m}^T\vec{q}+\lambda^2\norm{\vec{m}}^2+f_2&= 0 \\
\norm{\vec{q}}^2+2\lambda\vec{q}^T\vec{m}+\lambda^2\norm{\vec{m}}^2+f_2&= 0 
\end{align}
Taking $\lambda$ as common :
\begin{align}
\lambda(\lambda\norm{\vec{m}}^2+2\vec{q}^T\vec{m})&= -f_2-\norm{\vec{q}}^2\\
\lambda^2\norm{\vec{m}}^2&= -f_2-\norm{\vec{q}}^2\\
\lambda^2&= \frac{-f_2-\norm{\vec{q}}^2}{\norm{\vec{m}}^2} \\
\lambda^2&= \frac{3}{4} \\
\lambda&= +\sqrt{\frac{3}{4}},-\sqrt{\frac{3}{4}} \\
\lambda&= +\frac{\sqrt{3}}{2},-\frac{\sqrt{3}}{2} 
\end{align}
Substituting the value of $\lambda$ in \eqref{2.2.10}
\begin{align}
\vec{x}&= \vec{q}+\lambda\vec{m} \\
\vec{A}&= \myvec{\frac{1}{2} \\ \frac{\sqrt{3}}{2}} \\
\vec{B}&= \myvec{\frac{1}{2} \\ -\frac{\sqrt{3}}{2}}
\end{align} 
Now finding the direction vector $ \vec{m}_{O_1A}$,$\
\vec{m}_{O_1B}$,$ \vec{m}_{O_2A}$ and $\ \vec{m}_{O_2B}$.
\begin{align}
\vec{m}_{O_1A}=\myvec{1\\0}-\myvec{\frac{1}{2} \\ \frac{\sqrt{3}}{2}}&=\myvec{\frac{1}{2}\\-\frac{\sqrt{3}}{2}}\\
\vec{m}_{O_1B}=\myvec{1\\0}-\myvec{\frac{1}{2} \\ -\frac{\sqrt{3}}{2}}&=\myvec{\frac{1}{2}\\\frac{\sqrt{3}}{2}}\\
\vec{m}_{O_2A}=\myvec{0\\0}-\myvec{\frac{1}{2} \\ \frac{\sqrt{3}}{2}}&=\myvec{-\frac{1}{2}\\-\frac{\sqrt{3}}{2}}\\
\vec{m}_{O_2B}=\myvec{0\\0}-\myvec{\frac{1}{2} \\ -\frac{\sqrt{3}}{2}}&=\myvec{-\frac{1}{2}\\\frac{\sqrt{3}}{2}}
\end{align}
Now finding the angle $\angle{O_1AB}$.
\begin{align}
\vec{m}_{O_1A}^T \vec{m}_{O_1B}&=\norm{ \vec{m}_{O_1A}}\norm{\vec{m}_{O_1B}}\cos\theta_1\\
\frac{\vec{m}_{O_1A}^T \vec{m}_{O_1B}}{\norm{ \vec{m}_{O_1A}}\norm{\vec{m}_{O_1B}}}&=\cos\theta_1\\
\frac{-2}{4}&=\cos\theta_1\\
\frac{-1}{2}&=\cos\theta_1\\
\theta_1&=120^{\circ}
\end{align}
Now finding the angle $\angle{O_2AB}$.
\begin{align}
\vec{m}_{O_2A}^T \vec{m}_{O_2B}&=\norm{ \vec{m}_{O_2A}}\norm{\vec{m}_{O_2B}}\cos\theta_2\\
\frac{\vec{m}_{O_2A}^T \vec{m}_{O_2B}}{\norm{ \vec{m}_{O_2A}}\norm{\vec{m}_{O_2B}}}&=\cos\theta_2\\
\frac{-2}{4}&=\cos\theta_2\\
\frac{-1}{2}&=\cos\theta_2\\
\theta_2&=120^{\circ}
\end{align}
Finding area of $\bf{O_1AB}$ and $\bf{O_2AB}$.
 \begin{align}
A_{O_1AB}=\frac{\pi\theta_1}{360}r^2-\frac{1}{2}2\sqrt{3}\\
=\frac{120}{360}\pi-\frac{1}{2}2\sqrt{3}\\
A_{O_2AB}=\frac{\pi\theta_2}{360}r^2-\frac{1}{2}2\sqrt{3}\\
=\frac{120}{360}\pi-\frac{1}{2}2\sqrt{3}
\end{align}
Area of  $\bf{O_1AO_2B}$
\begin{align}
A_{O_1AO_2B}=\frac{120}{360}\pi-\frac{1}{2}2\sqrt{3}+\frac{120}{360}\pi-\frac{1}{2}2\sqrt{3}\\
=\frac{2\pi}{3}-2\sqrt{3}
\end{align}
\begin{figure}[h!]
\centering
\includegraphics[width=\columnwidth]{assignment4.JPG}
\caption{Figure depicting intersection points of circle}
\label{myfig}
\end{figure}
\end{document}